.

coq/theories/PetitSQL.v
@@ -205,13 +205,6 @@ Module P.
     - rewrite OBS_p_s. reflexivity.
   Qed.
 
-  Theorem some_spec {A : Type} (p : parser A) (p_isLt : isLt p)
-    : some p p_isLt == (p >>= fun x => some p p_isLt <|> pure [] >>= fun xs => pure (x :: xs)).
-  Proof.
-    intros s. rewrite some_unfold at 1. simpl. destruct (p s) as [[x s'] | ]; try reflexivity.
-    simpl. destruct (some p p_isLt s') as [[xs s''] | ]; try reflexivity.
-  Qed.
-
   Lemma some_isLt {A : Type} (p : parser A)
     (p_isLt : isLt p)
     : isLt (some p p_isLt).
@@ -220,6 +213,20 @@ Module P.
     assert (H_Acc : Acc (fun s1 : string => fun s2 : string => length s1 < length s2) s) by exact (Utils.acc_rel String.length lt Utils.acc_lt s).
     induction H_Acc as [s _ IH]. rewrite some_unfold. pose proof (p_isLt s) as length_s_gt_length_s'. destruct (p s) as [[x s'] | ]; trivial. specialize (IH s' length_s_gt_length_s'). destruct (some p p_isLt s') as [[xs s''] | ]; lia.
   Qed.
+
+  Definition many {A : Type} (p : parser A) (p_isLt : isLt p) : parser (list A) :=
+    some p p_isLt <|> pure [].
+
+  Theorem some_spec {A : Type} (p : parser A) (p_isLt : isLt p)
+    : some p p_isLt == (p >>= fun x => many p p_isLt >>= fun xs => pure (x :: xs)).
+  Proof.
+    intros s. rewrite some_unfold at 1. unfold many. simpl. destruct (p s) as [[x s'] | ]; try reflexivity.
+    simpl. destruct (some p p_isLt s') as [[xs s''] | ]; try reflexivity.
+  Qed.
+
+  Theorem many_spec {A : Type} (p : parser A) (p_isLt : isLt p)
+    : many p p_isLt == some p p_isLt <|> pure [].
+  Proof. reflexivity. Qed.
 
 End P.
 
